
[Back](../00.md)

## 2023-10-16

### Second Order Stochastic Dominance

Let $F_A(z), F_B(z)$ be two cumulative probability distributions for random payoffs in [a,b]. We say that $F_A(z)$ second order stochastically dominates (SSD) $F_B(z)$ if and only if:

$\int_a^z F_A(z) - F_B(z) dt , \leq 0,  \forall  z \in [a,b]$

($F_A$ is the function **below**)

---

### Theorem

Let $F_A(z), F_B(z)$ be two cumulative probability distributions for random payoffs in $[a,b]$. Than $F_A(z)$ second order stochastically dominates (SSD) $F_B(z)$ if and only if:

$E[u(A)] \geq E[u(B)]$ for all non-decreasing and concave utility functions $u$.

---

Exercise 4 SSD. Done on paper.

---

### Canonical Portfolio Problem

- Risk averse investor
- $Y_0$ = inital wealth
- Two investment opportunities:
  - One is risky with rate of return $\widetilde{r}$ 
  - One is risky-free with rate of return $rf$ 


$a$ = amount of money invested in the risky asset  
$Y_0-a$ = amount of money invested in the risk-free asset  

Time horizon is one period:

$\widetilde{Y} = (Y_0-a)(1+rf)+a(1+\widetilde{r}) = Y_0(1+rf)+a(1+\widetilde{r}-1-rf)\\$
$= Y_o(1+rf)+a(\widetilde{r}-rf)$

The investor chooses $a$ to maximize the expected utility of the final wealth $\widetilde{Y}$.


$\text{max } E[u(\widetilde{Y})] = \text{max } E[u(Y_o(1+rf)+a(\widetilde{r}-rf))]$

Wealth of $a$ = $W(a) = u(Y_o(1+rf)+a(\widetilde{r}-rf)) \\$


> Chain rule F(洧논) = f(g(洧논))  
> F'(洧논) = f'(g(洧논))*g'(洧논)  
> g(洧논) is the inner function and f(洧논) is the outer function. 

$W'(a) = E[u'(\widetilde{Y}(\widetilde{r}-rf))]$  
$W''(a) = E[u''(\widetilde{Y}(\widetilde{r}-rf)^2)] < 0 \space \forall \space a$

$\hat{a}$ is the solution of the maximization problem.  
In which condition is $\hat{a} > 0?$

---

If $W'(0) = 0$, tha maximum is in 0.  
This is the case in which $u$ is maximized when all the money is put in the risk free.

If $W'(0) < 0, \rightarrow \hat{a} < 0$  
If $W'(0) > 0, \rightarrow \hat{a} > 0$ 

---

Let's consider $W'(0) > 0$

$W'(0) = E[u'(\widetilde{Y}(\widetilde{r}-rf))] > 0$  

For this to be true:  
$u'(\widetilde{Y}(1+rf)) * E[\widetilde{r}-rf]> 0$  

We assume that $u'(\widetilde{Y}(1+rf))$ is an utility curve and therefore, $u'$ is positive.

So what we are left with is the following condition:  
$E[\widetilde{r}-rf]> 0$
 

